examples/low-level/crypto/Crypto.Symmetric.Chacha20.fst
@@ -1,250 +1,1696 @@
 module Crypto.Symmetric.Chacha20
 
-// Concrete implementation of CHACHA20 and countermode encryption
-// Not much point verifying its against a more complex pure specification.
 
-open FStar.Mul
-open FStar.Ghost
-(*  Machine integers *)
-open FStar.UInt8
-open FStar.UInt32
-open FStar.Int.Cast
-(*  Effects and memory layout *)
 open FStar.HyperStack
-(*  Buffers *)
+open FStar.ST
 open FStar.Buffer
-open Buffer.Utils
+open FStar.Int.Cast
+open FStar.UInt32
 
-module HH = FStar.HyperHeap
-module HS = FStar.HyperStack
+let u32 = FStar.UInt32.t
+let uint8_p = buffer FStar.UInt8.t
 
-type u64 = FStar.UInt64.t
-
-
-(*** Chacha 20 ***)
-
-inline_for_extraction let keylen   = 32ul
-inline_for_extraction let blocklen = 64ul 
-inline_for_extraction let ivlen    = 12ul
-
-type lbytes l = b:bytes {length b = l}
-type key   = lbytes (v keylen)
-type block = lbytes (v blocklen)
-type iv    = lbytes (v ivlen)
-
-// internally, blocks are represented as 16 x 4-byte integers
-private type matrix = m:uint32s{length m = v blocklen / 4}
-
-private type shuffle = 
-  m:matrix -> STL unit
-  (requires (fun h -> live h m))
-  (ensures (fun h0 _ h1 -> live h1 m /\ modifies_1 m h0 h1 ))
-
-(* lifted by hand for now: *)
-private val line:
-  m:matrix -> 
-  a:u32{v a < 16} -> 
-  b:u32{v b < 16} -> 
-  d:u32{v d < 16} -> 
-  s:u32{v s <= 32}-> STL unit
-  (requires (fun h -> live h m))
-  (ensures (fun h0 _ h1 -> live h1 m /\ modifies_1 m h0 h1 ))
-let line m a b d s = 
-  m.(a) <- m.(a) +%^ m.(b);
-  m.(d) <-(m.(d) ^^  m.(a)) <<< s
-
-private val quarter_round:
-  m:matrix -> 
-  a:u32{v a < 16} -> 
-  b:u32{v b < 16} -> 
-  c:u32{v c < 16} -> 
-  d:u32{v d < 16} -> STL unit
-  (requires (fun h -> live h m))
-  (ensures (fun h0 _ h1 -> live h1 m /\ modifies_1 m h0 h1 ))
-let quarter_round m a b c d = 
-(*
-  let line a b d s = 
-    upd m a (m.(a) +%^ m.(b));
-    upd m d((m.(d) ^^  m.(a)) <<< s) in
-*)    
-  line m a b d 16ul;
-  line m c d b 12ul;
-  line m a b d  8ul; 
-  line m c d b  7ul
-
-private val column_round: shuffle 
-let column_round m =
-  quarter_round m 0ul 4ul  8ul 12ul;
-  quarter_round m 1ul 5ul  9ul 13ul;
-  quarter_round m 2ul 6ul 10ul 14ul;
-  quarter_round m 3ul 7ul 11ul 15ul
-
-private val diagonal_round: shuffle
-let diagonal_round m =
-  quarter_round m 0ul 5ul 10ul 15ul;
-  quarter_round m 1ul 6ul 11ul 12ul;
-  quarter_round m 2ul 7ul  8ul 13ul;
-  quarter_round m 3ul 4ul  9ul 14ul
-
-private val rounds: shuffle 
-let rounds m = (* 20 rounds *)
-  column_round m; diagonal_round m; 
-  column_round m; diagonal_round m;
-  column_round m; diagonal_round m;
-  column_round m; diagonal_round m;
-  column_round m; diagonal_round m;
-  column_round m; diagonal_round m;
-  column_round m; diagonal_round m;
-  column_round m; diagonal_round m;
-  column_round m; diagonal_round m;
-  column_round m; diagonal_round m
-
-private val chacha20_init: 
-  m:matrix -> k:key{disjoint m k} -> n:iv{disjoint m n} -> counter:u32 -> 
-  STL unit
-  (requires (fun h -> live h m /\ live h k /\ live h n ))
-  (ensures (fun h0 _ h1 -> live h1 m /\ modifies_1 m h0 h1))
-
-private val fill: m:matrix -> i:u32 -> len:u32 {v i + v len <= 16}-> src:bytes {length src = 4 * v len} -> 
-  STL unit
-  (requires (fun h -> live h m /\ live h src /\ disjoint m src))
-  (ensures (fun h0 _ h1 -> live h1 m /\ modifies_1 m h0 h1))
-let rec fill m i len src =
-  if len <> 0ul then (
-    m.(i) <- uint32_of_bytes (sub src 0ul 4ul); 
-    let len = len -^ 1ul in 
-    fill m (i +^ 1ul) len (sub src 4ul (4ul *^ len)))
-
-//review handling of endianness
-
-// RFC 7539 2.3
-let chacha20_init m key iv counter =
-  m.(0ul) <- 0x61707865ul;
-  m.(1ul) <- 0x3320646eul;
-  m.(2ul) <- 0x79622d32ul;
-  m.(3ul) <- 0x6b206574ul;
-  fill m 4ul 8ul key;
-  m.(12ul) <- counter; 
-  fill m 13ul 3ul iv
-
-(* lifted by hand for now: *)
-private val add: 
-  m: matrix -> m0: matrix{disjoint m m0} -> 
-  i:u32 { i <^ 16ul } ->
-  STL unit
-  (requires (fun h -> live h m /\ live h m0))
-  (ensures (fun h0 _ h1 -> live h1 m /\ modifies_1 m h0 h1))
-let add m m0 i = 
-  m.(i) <- m.(i) +%^ m0.(i)
-
-private val sum_matrixes: 
-  m: matrix -> m0:matrix{disjoint m m0} -> 
-  STL unit
-  (requires (fun h -> live h m /\ live h m0))
-  (ensures (fun h0 _ h1 -> live h1 m /\ modifies_1 m h0 h1))
-let sum_matrixes m m0 =
-//let add i = upd m i (m.(i) +%^ m0.(i)) in // inlined? 
-// forUint32 0ul 15ul (fun i -> add m m0 i)
-  add m m0  0ul;
-  add m m0  1ul;
-  add m m0  2ul;
-  add m m0  3ul;
-  add m m0  4ul;
-  add m m0  5ul;
-  add m m0  6ul;
-  add m m0  7ul;
-  add m m0  8ul;
-  add m m0  9ul;
-  add m m0 10ul;
-  add m m0 11ul;
-  add m m0 12ul;
-  add m m0 13ul;
-  add m m0 14ul;
-  add m m0 15ul
-
-private val chacha20_update: 
-  output:bytes -> 
-  state:uint32s{length state = 32 /\ disjoint state output} ->
-  len:u32{v len <= 64 /\ length output >= v len} -> STL unit
-    (requires (fun h -> live h state /\ live h output))
-    (ensures (fun h0 _ h1 -> live h1 output /\ live h1 state /\ modifies_2 output state h0 h1 ))
-let chacha20_update output state len =
-  (* Initial state *) 
-  let m  = sub state  0ul 16ul in
-  let m0 = sub state 16ul 16ul in // do we ever rely on m and m0 being contiguous?
-  blit m 0ul m0 0ul 16ul;
-  rounds m;
-  (* Sum the matrixes *)
-  sum_matrixes m m0;
-  (* Serialize the state into byte stream *)
-  bytes_of_uint32s output m len
-// avoid this copy when XORing? merge the sum_matrix and output loops? we don't use m0 afterward. 
-
-// computes one pseudo-random 64-byte block 
-// (consider fixing len to 64ul)
-
-val chacha20: 
-  output:bytes -> 
-  k:key ->
-  n:iv ->
-  counter: u32 ->
-  len:u32{v len <= v blocklen /\ v len <= length output} -> STL unit
-    (requires (fun h -> live h k /\ live h n /\ live h output))
-    (ensures (fun h0 _ h1 -> live h1 output /\ modifies_1 output h0 h1 ))
-let chacha20 output key n counter len = 
-  push_frame ();
-  let state = create 0ul 32ul in
-  let m = sub state 0ul 16ul in
-  chacha20_init m key n counter;
-  chacha20_update output state len;
-  pop_frame ()
-
-// Performance: it may be easier to precompute and re-use an expanded key (m0), 
-// to avoid passing around (key, counter, iv, constant), and only have m on the stack.
-// We may also merge the 3 final loops: sum_matrixes, bytes_of_uint32s, and outer XOR/ADD. 
+type chacha_ctx = b:Buffer.buffer u32{length b = 16}
 
 
-(*** Counter-mode Encryption ***)
+val lemma_max_uint32: n:nat -> 
+  Lemma (requires (n = 32))
+        (ensures (pow2 n = 4294967296))
+        [SMTPat (pow2 n)]
+let lemma_max_uint32 n = assert_norm (pow2 32 = 4294967296)
 
-// The rest of this code is not specific to chacha20.
-// It is parameterized by the initial counter (0, or 1 for some AEAD)
-// and the block length (here 64 bytes).
-// It should appear after PRF idealization.
+let op_Less_Less_Less (a:u32) (s:u32{FStar.UInt32.v s <= 32}) : Tot u32 =
+  (a <<^ s) |^ (a >>^ (FStar.UInt32 (32ul -^ s)))
 
-private let prf = chacha20
 
-// XOR-based encryption and decryption (just swap ciphertext and plaintext)
-val counter_mode: 
-  k:key -> n:iv -> counter:u32 -> 
-  len:u32{v counter + v len / v blocklen < pow2 32} ->
-  plaintext:bytes {length plaintext = v len /\ disjoint k plaintext} -> 
-  ciphertext:bytes {length ciphertext = v len /\ disjoint n ciphertext /\ disjoint k ciphertext /\ disjoint plaintext ciphertext} -> 
-  STL unit
-    (requires (fun h -> live h ciphertext /\ live h k /\ live h n /\ live h plaintext))
-    (ensures (fun h0 _ h1 -> live h1 ciphertext /\ modifies_1 ciphertext h0 h1))
+#reset-options "--initial_fuel 0 --max_fuel 0 --z3timeout 5"
 
-#reset-options "--z3timeout 100"
-// a bit slow, e.g. on the len precondition
+let load32_le (k:uint8_p) : Stack u32
+  (requires (fun h -> live h k /\ length k >= 4))
+  (ensures  (fun h0 _ h1 -> h0 == h1))
+  = let k0 = k.(0ul) in
+    let k1 = k.(1ul) in
+    let k2 = k.(2ul) in
+    let k3 = k.(3ul) in
+    let z = uint8_to_uint32 k0
+            |^ (uint8_to_uint32 k1 <<^ 8ul)
+            |^ (uint8_to_uint32 k2 <<^ 16ul)
+            |^ (uint8_to_uint32 k3 <<^ 24ul) in
+    z
 
-let rec counter_mode key iv counter len plaintext ciphertext =
-  if len =^ 0ul then () 
-  else if len <^ blocklen 
-  then (* encrypt final partial block *)
-    begin
-      let cipher = sub ciphertext  0ul len in 
-      let plain  = sub plaintext   0ul len in 
-      prf cipher key iv counter len;
-      xor_bytes_inplace cipher plain len
-    end
-  else (* encrypt full block *)
-    begin
-      let cipher = sub ciphertext  0ul blocklen in
-      let plain  = sub plaintext   0ul blocklen in
-      prf cipher key iv counter blocklen;
-      xor_bytes_inplace cipher plain blocklen;
-      let len = len -^ blocklen in
-      let ciphertext = sub ciphertext blocklen len in
-      let plaintext  = sub plaintext  blocklen len in
-      counter_mode key iv (counter +^ 1ul) len plaintext ciphertext
-    end
+let store32_le (k:uint8_p) (x:u32) : Stack unit
+  (requires (fun h -> live h k /\ length k >= 4))
+  (ensures  (fun h0 _ h1 -> modifies_1 k h0 h1 /\ live h1 k))
+  = k.(0ul) <- uint32_to_uint8 x;
+    k.(1ul) <- uint32_to_uint8 (x >>^ 8ul);
+    k.(2ul) <- uint32_to_uint8 (x >>^ 16ul);
+    k.(3ul) <- uint32_to_uint8 (x >>^ 24ul)
+
+
+val quarter_round:
+  m:chacha_ctx ->
+  a:u32{FStar.UInt32.v a < 16} ->
+  b:u32{FStar.UInt32.v b<16} ->
+  c:u32{FStar.UInt32.v c<16} ->
+  d:u32{FStar.UInt32.v d<16} ->
+  Stack unit
+    (requires (fun h -> live h m))
+    (ensures (fun h0 _ h1 -> live h1 m /\ modifies_1 m h0 h1))
+let quarter_round m a b c d =
+  let ma = m.(a) in let mb = m.(b) in m.(a) <- (ma +%^ mb);
+  let md = m.(d) in let ma = m.(a) in m.(d) <- (md ^^ ma);
+  let md = m.(d) in                   m.(d) <- (md <<< 16ul);
+  let mc = m.(c) in let md = m.(d) in m.(c) <- (mc +%^ md);
+  let mb = m.(b) in let mc = m.(c) in m.(b) <- (mb ^^ mc);
+  let mb = m.(b) in                   m.(b) <- (mb <<< 12ul);
+  let ma = m.(a) in let mb = m.(b) in m.(a) <- (ma +%^ mb);
+  let md = m.(d) in let ma = m.(a) in m.(d) <- (md ^^ ma);
+  let md = m.(d) in                   m.(d) <- (md <<< 8ul);
+  let mc = m.(c) in let md = m.(d) in m.(c) <- (mc +%^ md);
+  let mb = m.(b) in let mc = m.(c) in m.(b) <- (mb ^^ mc);
+  let mb = m.(b) in                   m.(b) <- (mb <<< 7ul)
+
+
+val chacha_keysetup:
+  ctx:chacha_ctx ->
+  k:uint8_p ->
+  Stack unit
+    (requires (fun _ -> True))
+    (ensures  (fun _ _ _ -> True))
+let chacha_keysetup ctx k =
+    ctx.(0ul)  <- (0x61707865ul);
+    ctx.(1ul)  <- (0x3320646eul);
+    ctx.(2ul)  <- (0x79622d32ul);
+    ctx.(3ul)  <- (0x6b206574ul);
+    ctx.(4ul)  <- load32_le(offset k  0ul);
+    ctx.(5ul)  <- load32_le(offset k  4ul);
+    ctx.(6ul)  <- load32_le(offset k  8ul);
+    ctx.(7ul)  <- load32_le(offset k 12ul);
+    ctx.(8ul)  <- load32_le(offset k 16ul);
+    ctx.(9ul)  <- load32_le(offset k 20ul);
+    ctx.(10ul) <- load32_le(offset k 24ul);
+    ctx.(11ul) <- load32_le(offset k 28ul)
+
+
+val chacha_ivsetup:
+  ctx:chacha_ctx ->
+  k:uint8_p ->
+  counter:uint8_p ->
+  Stack unit
+    (requires (fun _ -> True))
+    (ensures  (fun _ _ _ -> True))
+let chacha_ivsetup ctx iv counter =
+    ctx.(12ul) <- load32_le(counter);
+    ctx.(13ul) <- load32_le(offset counter 4ul);
+    ctx.(14ul) <- load32_le(iv);
+    ctx.(15ul) <- load32_le(offset iv 4ul)
+
+
+val chacha_ietf_ivsetup:
+  ctx:chacha_ctx ->
+  k:uint8_p ->
+  counter:u32 ->
+  Stack unit
+    (requires (fun _ -> True))
+    (ensures  (fun _ _ _ -> True))
+let chacha_ietf_ivsetup ctx iv counter =
+    ctx.(12ul) <- counter;
+    ctx.(13ul) <- load32_le(iv);
+    ctx.(14ul) <- load32_le(offset iv 4ul);
+    ctx.(15ul) <- load32_le(offset iv 8ul)
+
+
+val chacha_encrypt_bytes_core:
+  ctx:chacha_ctx ->
+  m:uint8_p ->
+  c:uint8_p ->
+  Stack unit
+    (requires (fun _ -> True))
+    (ensures  (fun _ _ _ -> True))
+let chacha_encrypt_bytes_core ctx m c =
+  let j0 = ctx.(0ul) in
+  let j1 = ctx.(1ul) in
+  let j2 = ctx.(2ul) in
+  let j3 = ctx.(3ul) in
+  let j4 = ctx.(4ul) in
+  let j5 = ctx.(5ul) in
+  let j6 = ctx.(6ul) in
+  let j7 = ctx.(7ul) in
+  let j8 = ctx.(8ul) in
+  let j9 = ctx.(9ul) in
+  let j10 = ctx.(10ul) in
+  let j11 = ctx.(11ul) in
+  let j12 = ctx.(12ul) in
+  let j13 = ctx.(13ul) in
+  let j14 = ctx.(14ul) in
+  let j15 = ctx.(15ul) in
+
+  (* let x = Buffer.sub ctx 16ul 16ul in *)
+  (* let ctx = Buffer.sub ctx 0ul 16ul in *)
+  (* blit ctx 0ul x 0ul 16ul; *)
+
+  (* quarter_round x 0ul 4ul 8ul 12ul; *)
+  (* quarter_round x 1ul 5ul 9ul 13ul; *)
+  (* quarter_round x 2ul 6ul 10ul 14ul; *)
+  (* quarter_round x 3ul 7ul 11ul 15ul; *)
+  (* quarter_round x 0ul 5ul 10ul 15ul; *)
+  (* quarter_round x 1ul 6ul 11ul 12ul; *)
+  (* quarter_round x 2ul 7ul 8ul 13ul; *)
+  (* quarter_round x 3ul 4ul 9ul 14ul;   *)
+
+  (* quarter_round x 0ul 4ul 8ul 12ul; *)
+  (* quarter_round x 1ul 5ul 9ul 13ul; *)
+  (* quarter_round x 2ul 6ul 10ul 14ul; *)
+  (* quarter_round x 3ul 7ul 11ul 15ul; *)
+  (* quarter_round x 0ul 5ul 10ul 15ul; *)
+  (* quarter_round x 1ul 6ul 11ul 12ul; *)
+  (* quarter_round x 2ul 7ul 8ul 13ul; *)
+  (* quarter_round x 3ul 4ul 9ul 14ul;   *)
+
+  (* quarter_round x 0ul 4ul 8ul 12ul; *)
+  (* quarter_round x 1ul 5ul 9ul 13ul; *)
+  (* quarter_round x 2ul 6ul 10ul 14ul; *)
+  (* quarter_round x 3ul 7ul 11ul 15ul; *)
+  (* quarter_round x 0ul 5ul 10ul 15ul; *)
+  (* quarter_round x 1ul 6ul 11ul 12ul; *)
+  (* quarter_round x 2ul 7ul 8ul 13ul; *)
+  (* quarter_round x 3ul 4ul 9ul 14ul;   *)
+
+  (* quarter_round x 0ul 4ul 8ul 12ul; *)
+  (* quarter_round x 1ul 5ul 9ul 13ul; *)
+  (* quarter_round x 2ul 6ul 10ul 14ul; *)
+  (* quarter_round x 3ul 7ul 11ul 15ul; *)
+  (* quarter_round x 0ul 5ul 10ul 15ul; *)
+  (* quarter_round x 1ul 6ul 11ul 12ul; *)
+  (* quarter_round x 2ul 7ul 8ul 13ul; *)
+  (* quarter_round x 3ul 4ul 9ul 14ul;   *)
+
+  (* quarter_round x 0ul 4ul 8ul 12ul; *)
+  (* quarter_round x 1ul 5ul 9ul 13ul; *)
+  (* quarter_round x 2ul 6ul 10ul 14ul; *)
+  (* quarter_round x 3ul 7ul 11ul 15ul; *)
+  (* quarter_round x 0ul 5ul 10ul 15ul; *)
+  (* quarter_round x 1ul 6ul 11ul 12ul; *)
+  (* quarter_round x 2ul 7ul 8ul 13ul; *)
+  (* quarter_round x 3ul 4ul 9ul 14ul;   *)
+
+  (* quarter_round x 0ul 4ul 8ul 12ul; *)
+  (* quarter_round x 1ul 5ul 9ul 13ul; *)
+  (* quarter_round x 2ul 6ul 10ul 14ul; *)
+  (* quarter_round x 3ul 7ul 11ul 15ul; *)
+  (* quarter_round x 0ul 5ul 10ul 15ul; *)
+  (* quarter_round x 1ul 6ul 11ul 12ul; *)
+  (* quarter_round x 2ul 7ul 8ul 13ul; *)
+  (* quarter_round x 3ul 4ul 9ul 14ul;   *)
+
+  (* quarter_round x 0ul 4ul 8ul 12ul; *)
+  (* quarter_round x 1ul 5ul 9ul 13ul; *)
+  (* quarter_round x 2ul 6ul 10ul 14ul; *)
+  (* quarter_round x 3ul 7ul 11ul 15ul; *)
+  (* quarter_round x 0ul 5ul 10ul 15ul; *)
+  (* quarter_round x 1ul 6ul 11ul 12ul; *)
+  (* quarter_round x 2ul 7ul 8ul 13ul; *)
+  (* quarter_round x 3ul 4ul 9ul 14ul;   *)
+
+  (* quarter_round x 0ul 4ul 8ul 12ul; *)
+  (* quarter_round x 1ul 5ul 9ul 13ul; *)
+  (* quarter_round x 2ul 6ul 10ul 14ul; *)
+  (* quarter_round x 3ul 7ul 11ul 15ul; *)
+  (* quarter_round x 0ul 5ul 10ul 15ul; *)
+  (* quarter_round x 1ul 6ul 11ul 12ul; *)
+  (* quarter_round x 2ul 7ul 8ul 13ul; *)
+  (* quarter_round x 3ul 4ul 9ul 14ul;   *)
+
+  (* quarter_round x 0ul 4ul 8ul 12ul; *)
+  (* quarter_round x 1ul 5ul 9ul 13ul; *)
+  (* quarter_round x 2ul 6ul 10ul 14ul; *)
+  (* quarter_round x 3ul 7ul 11ul 15ul; *)
+  (* quarter_round x 0ul 5ul 10ul 15ul; *)
+  (* quarter_round x 1ul 6ul 11ul 12ul; *)
+  (* quarter_round x 2ul 7ul 8ul 13ul; *)
+  (* quarter_round x 3ul 4ul 9ul 14ul;   *)
+
+  (* quarter_round x 0ul 4ul 8ul 12ul; *)
+  (* quarter_round x 1ul 5ul 9ul 13ul; *)
+  (* quarter_round x 2ul 6ul 10ul 14ul; *)
+  (* quarter_round x 3ul 7ul 11ul 15ul; *)
+  (* quarter_round x 0ul 5ul 10ul 15ul; *)
+  (* quarter_round x 1ul 6ul 11ul 12ul; *)
+  (* quarter_round x 2ul 7ul 8ul 13ul; *)
+  (* quarter_round x 3ul 4ul 9ul 14ul;   *)
+
+  let x0 = j0 in
+  let x1 = j1 in
+  let x2 = j2 in
+  let x3 = j3 in
+  let x4 = j4 in
+  let x5 = j5 in
+  let x6 = j6 in
+  let x7 = j7 in
+  let x8 = j8 in
+  let x9 = j9 in
+  let x10 = j10 in
+  let x11 = j11 in
+  let x12 = j12 in
+  let x13 = j13 in
+  let x14 = j14 in
+  let x15 = j15 in
+
+  let x0 = x0 +%^ x4 in
+  let x12 = x12 ^^ x0 in
+  let x12 = x12 <<< 16ul in
+  let x8 = x8 +%^ x12 in
+  let x4 = x4 ^^ x8 in
+  let x4 = x4 <<< 12ul in
+  let x0 = x0 +%^ x4 in
+  let x12 = x12 ^^ x0 in
+  let x12 = x12 <<< 8ul in
+  let x8 = x8 +%^ x12 in
+  let x4 = x4 ^^ x8 in
+  let x4 = x4 <<< 7ul in
+
+  let x1 = x1 +%^ x5 in
+  let x13 = x13 ^^ x1 in
+  let x13 = x13 <<< 16ul in
+  let x9 = x9 +%^ x13 in
+  let x5 = x5 ^^ x9 in
+  let x5 = x5 <<< 12ul in
+  let x1 = x1 +%^ x5 in
+  let x13 = x13 ^^ x1 in
+  let x13 = x13 <<< 8ul in
+  let x9 = x9 +%^ x13 in
+  let x5 = x5 ^^ x9 in
+  let x5 = x5 <<< 7ul in
+
+  let x2 = x2 +%^ x6 in
+  let x14 = x14 ^^ x2 in
+  let x14 = x14 <<< 16ul in
+  let x10 = x10 +%^ x14 in
+  let x6 = x6 ^^ x10 in
+  let x6 = x6 <<< 12ul in
+  let x2 = x2 +%^ x6 in
+  let x14 = x14 ^^ x2 in
+  let x14 = x14 <<< 8ul in
+  let x10 = x10 +%^ x14 in
+  let x6 = x6 ^^ x10 in
+  let x6 = x6 <<< 7ul in
+
+  let x3 = x3 +%^ x7 in
+  let x15 = x15 ^^ x3 in
+  let x15 = x15 <<< 16ul in
+  let x11 = x11 +%^ x15 in
+  let x7 = x7 ^^ x11 in
+  let x7 = x7 <<< 12ul in
+  let x3 = x3 +%^ x7 in
+  let x15 = x15 ^^ x3 in
+  let x15 = x15 <<< 8ul in
+  let x11 = x11 +%^ x15 in
+  let x7 = x7 ^^ x11 in
+  let x7 = x7 <<< 7ul in
+
+  let x0 = x0 +%^ x5 in
+  let x15 = x15 ^^ x0 in
+  let x15 = x15 <<< 16ul in
+  let x10 = x10 +%^ x15 in
+  let x5 = x5 ^^ x10 in
+  let x5 = x5 <<< 12ul in
+  let x0 = x0 +%^ x5 in
+  let x15 = x15 ^^ x0 in
+  let x15 = x15 <<< 8ul in
+  let x10 = x10 +%^ x15 in
+  let x5 = x5 ^^ x10 in
+  let x5 = x5 <<< 7ul in
+
+  let x1 = x1 +%^ x6 in
+  let x12 = x12 ^^ x1 in
+  let x12 = x12 <<< 16ul in
+  let x11 = x11 +%^ x12 in
+  let x6 = x6 ^^ x11 in
+  let x6 = x6 <<< 12ul in
+  let x1 = x1 +%^ x6 in
+  let x12 = x12 ^^ x1 in
+  let x12 = x12 <<< 8ul in
+  let x11 = x11 +%^ x12 in
+  let x6 = x6 ^^ x11 in
+  let x6 = x6 <<< 7ul in
+
+  let x2 = x2 +%^ x7 in
+  let x13 = x13 ^^ x2 in
+  let x13 = x13 <<< 16ul in
+  let x8 = x8 +%^ x13 in
+  let x7 = x7 ^^ x8 in
+  let x7 = x7 <<< 12ul in
+  let x2 = x2 +%^ x7 in
+  let x13 = x13 ^^ x2 in
+  let x13 = x13 <<< 8ul in
+  let x8 = x8 +%^ x13 in
+  let x7 = x7 ^^ x8 in
+  let x7 = x7 <<< 7ul in
+
+  let x3 = x3 +%^ x4 in
+  let x14 = x14 ^^ x3 in
+  let x14 = x14 <<< 16ul in
+  let x9 = x9 +%^ x14 in
+  let x4 = x4 ^^ x9 in
+  let x4 = x4 <<< 12ul in
+  let x3 = x3 +%^ x4 in
+  let x14 = x14 ^^ x3 in
+  let x14 = x14 <<< 8ul in
+  let x9 = x9 +%^ x14 in
+  let x4 = x4 ^^ x9 in
+  let x4 = x4 <<< 7ul in
+
+  (* 1 *)
+
+  let x0 = x0 +%^ x4 in
+  let x12 = x12 ^^ x0 in
+  let x12 = x12 <<< 16ul in
+  let x8 = x8 +%^ x12 in
+  let x4 = x4 ^^ x8 in
+  let x4 = x4 <<< 12ul in
+  let x0 = x0 +%^ x4 in
+  let x12 = x12 ^^ x0 in
+  let x12 = x12 <<< 8ul in
+  let x8 = x8 +%^ x12 in
+  let x4 = x4 ^^ x8 in
+  let x4 = x4 <<< 7ul in
+
+  let x1 = x1 +%^ x5 in
+  let x13 = x13 ^^ x1 in
+  let x13 = x13 <<< 16ul in
+  let x9 = x9 +%^ x13 in
+  let x5 = x5 ^^ x9 in
+  let x5 = x5 <<< 12ul in
+  let x1 = x1 +%^ x5 in
+  let x13 = x13 ^^ x1 in
+  let x13 = x13 <<< 8ul in
+  let x9 = x9 +%^ x13 in
+  let x5 = x5 ^^ x9 in
+  let x5 = x5 <<< 7ul in
+
+  let x2 = x2 +%^ x6 in
+  let x14 = x14 ^^ x2 in
+  let x14 = x14 <<< 16ul in
+  let x10 = x10 +%^ x14 in
+  let x6 = x6 ^^ x10 in
+  let x6 = x6 <<< 12ul in
+  let x2 = x2 +%^ x6 in
+  let x14 = x14 ^^ x2 in
+  let x14 = x14 <<< 8ul in
+  let x10 = x10 +%^ x14 in
+  let x6 = x6 ^^ x10 in
+  let x6 = x6 <<< 7ul in
+
+  let x3 = x3 +%^ x7 in
+  let x15 = x15 ^^ x3 in
+  let x15 = x15 <<< 16ul in
+  let x11 = x11 +%^ x15 in
+  let x7 = x7 ^^ x11 in
+  let x7 = x7 <<< 12ul in
+  let x3 = x3 +%^ x7 in
+  let x15 = x15 ^^ x3 in
+  let x15 = x15 <<< 8ul in
+  let x11 = x11 +%^ x15 in
+  let x7 = x7 ^^ x11 in
+  let x7 = x7 <<< 7ul in
+
+  let x0 = x0 +%^ x5 in
+  let x15 = x15 ^^ x0 in
+  let x15 = x15 <<< 16ul in
+  let x10 = x10 +%^ x15 in
+  let x5 = x5 ^^ x10 in
+  let x5 = x5 <<< 12ul in
+  let x0 = x0 +%^ x5 in
+  let x15 = x15 ^^ x0 in
+  let x15 = x15 <<< 8ul in
+  let x10 = x10 +%^ x15 in
+  let x5 = x5 ^^ x10 in
+  let x5 = x5 <<< 7ul in
+
+  let x1 = x1 +%^ x6 in
+  let x12 = x12 ^^ x1 in
+  let x12 = x12 <<< 16ul in
+  let x11 = x11 +%^ x12 in
+  let x6 = x6 ^^ x11 in
+  let x6 = x6 <<< 12ul in
+  let x1 = x1 +%^ x6 in
+  let x12 = x12 ^^ x1 in
+  let x12 = x12 <<< 8ul in
+  let x11 = x11 +%^ x12 in
+  let x6 = x6 ^^ x11 in
+  let x6 = x6 <<< 7ul in
+
+  let x2 = x2 +%^ x7 in
+  let x13 = x13 ^^ x2 in
+  let x13 = x13 <<< 16ul in
+  let x8 = x8 +%^ x13 in
+  let x7 = x7 ^^ x8 in
+  let x7 = x7 <<< 12ul in
+  let x2 = x2 +%^ x7 in
+  let x13 = x13 ^^ x2 in
+  let x13 = x13 <<< 8ul in
+  let x8 = x8 +%^ x13 in
+  let x7 = x7 ^^ x8 in
+  let x7 = x7 <<< 7ul in
+
+  let x3 = x3 +%^ x4 in
+  let x14 = x14 ^^ x3 in
+  let x14 = x14 <<< 16ul in
+  let x9 = x9 +%^ x14 in
+  let x4 = x4 ^^ x9 in
+  let x4 = x4 <<< 12ul in
+  let x3 = x3 +%^ x4 in
+  let x14 = x14 ^^ x3 in
+  let x14 = x14 <<< 8ul in
+  let x9 = x9 +%^ x14 in
+  let x4 = x4 ^^ x9 in
+  let x4 = x4 <<< 7ul in
+
+  (* 2 *)
+
+  let x0 = x0 +%^ x4 in
+  let x12 = x12 ^^ x0 in
+  let x12 = x12 <<< 16ul in
+  let x8 = x8 +%^ x12 in
+  let x4 = x4 ^^ x8 in
+  let x4 = x4 <<< 12ul in
+  let x0 = x0 +%^ x4 in
+  let x12 = x12 ^^ x0 in
+  let x12 = x12 <<< 8ul in
+  let x8 = x8 +%^ x12 in
+  let x4 = x4 ^^ x8 in
+  let x4 = x4 <<< 7ul in
+
+  let x1 = x1 +%^ x5 in
+  let x13 = x13 ^^ x1 in
+  let x13 = x13 <<< 16ul in
+  let x9 = x9 +%^ x13 in
+  let x5 = x5 ^^ x9 in
+  let x5 = x5 <<< 12ul in
+  let x1 = x1 +%^ x5 in
+  let x13 = x13 ^^ x1 in
+  let x13 = x13 <<< 8ul in
+  let x9 = x9 +%^ x13 in
+  let x5 = x5 ^^ x9 in
+  let x5 = x5 <<< 7ul in
+
+  let x2 = x2 +%^ x6 in
+  let x14 = x14 ^^ x2 in
+  let x14 = x14 <<< 16ul in
+  let x10 = x10 +%^ x14 in
+  let x6 = x6 ^^ x10 in
+  let x6 = x6 <<< 12ul in
+  let x2 = x2 +%^ x6 in
+  let x14 = x14 ^^ x2 in
+  let x14 = x14 <<< 8ul in
+  let x10 = x10 +%^ x14 in
+  let x6 = x6 ^^ x10 in
+  let x6 = x6 <<< 7ul in
+
+  let x3 = x3 +%^ x7 in
+  let x15 = x15 ^^ x3 in
+  let x15 = x15 <<< 16ul in
+  let x11 = x11 +%^ x15 in
+  let x7 = x7 ^^ x11 in
+  let x7 = x7 <<< 12ul in
+  let x3 = x3 +%^ x7 in
+  let x15 = x15 ^^ x3 in
+  let x15 = x15 <<< 8ul in
+  let x11 = x11 +%^ x15 in
+  let x7 = x7 ^^ x11 in
+  let x7 = x7 <<< 7ul in
+
+  let x0 = x0 +%^ x5 in
+  let x15 = x15 ^^ x0 in
+  let x15 = x15 <<< 16ul in
+  let x10 = x10 +%^ x15 in
+  let x5 = x5 ^^ x10 in
+  let x5 = x5 <<< 12ul in
+  let x0 = x0 +%^ x5 in
+  let x15 = x15 ^^ x0 in
+  let x15 = x15 <<< 8ul in
+  let x10 = x10 +%^ x15 in
+  let x5 = x5 ^^ x10 in
+  let x5 = x5 <<< 7ul in
+
+  let x1 = x1 +%^ x6 in
+  let x12 = x12 ^^ x1 in
+  let x12 = x12 <<< 16ul in
+  let x11 = x11 +%^ x12 in
+  let x6 = x6 ^^ x11 in
+  let x6 = x6 <<< 12ul in
+  let x1 = x1 +%^ x6 in
+  let x12 = x12 ^^ x1 in
+  let x12 = x12 <<< 8ul in
+  let x11 = x11 +%^ x12 in
+  let x6 = x6 ^^ x11 in
+  let x6 = x6 <<< 7ul in
+
+  let x2 = x2 +%^ x7 in
+  let x13 = x13 ^^ x2 in
+  let x13 = x13 <<< 16ul in
+  let x8 = x8 +%^ x13 in
+  let x7 = x7 ^^ x8 in
+  let x7 = x7 <<< 12ul in
+  let x2 = x2 +%^ x7 in
+  let x13 = x13 ^^ x2 in
+  let x13 = x13 <<< 8ul in
+  let x8 = x8 +%^ x13 in
+  let x7 = x7 ^^ x8 in
+  let x7 = x7 <<< 7ul in
+
+  let x3 = x3 +%^ x4 in
+  let x14 = x14 ^^ x3 in
+  let x14 = x14 <<< 16ul in
+  let x9 = x9 +%^ x14 in
+  let x4 = x4 ^^ x9 in
+  let x4 = x4 <<< 12ul in
+  let x3 = x3 +%^ x4 in
+  let x14 = x14 ^^ x3 in
+  let x14 = x14 <<< 8ul in
+  let x9 = x9 +%^ x14 in
+  let x4 = x4 ^^ x9 in
+  let x4 = x4 <<< 7ul in
+
+  (* 3 *)
+
+  let x0 = x0 +%^ x4 in
+  let x12 = x12 ^^ x0 in
+  let x12 = x12 <<< 16ul in
+  let x8 = x8 +%^ x12 in
+  let x4 = x4 ^^ x8 in
+  let x4 = x4 <<< 12ul in
+  let x0 = x0 +%^ x4 in
+  let x12 = x12 ^^ x0 in
+  let x12 = x12 <<< 8ul in
+  let x8 = x8 +%^ x12 in
+  let x4 = x4 ^^ x8 in
+  let x4 = x4 <<< 7ul in
+
+  let x1 = x1 +%^ x5 in
+  let x13 = x13 ^^ x1 in
+  let x13 = x13 <<< 16ul in
+  let x9 = x9 +%^ x13 in
+  let x5 = x5 ^^ x9 in
+  let x5 = x5 <<< 12ul in
+  let x1 = x1 +%^ x5 in
+  let x13 = x13 ^^ x1 in
+  let x13 = x13 <<< 8ul in
+  let x9 = x9 +%^ x13 in
+  let x5 = x5 ^^ x9 in
+  let x5 = x5 <<< 7ul in
+
+  let x2 = x2 +%^ x6 in
+  let x14 = x14 ^^ x2 in
+  let x14 = x14 <<< 16ul in
+  let x10 = x10 +%^ x14 in
+  let x6 = x6 ^^ x10 in
+  let x6 = x6 <<< 12ul in
+  let x2 = x2 +%^ x6 in
+  let x14 = x14 ^^ x2 in
+  let x14 = x14 <<< 8ul in
+  let x10 = x10 +%^ x14 in
+  let x6 = x6 ^^ x10 in
+  let x6 = x6 <<< 7ul in
+
+  let x3 = x3 +%^ x7 in
+  let x15 = x15 ^^ x3 in
+  let x15 = x15 <<< 16ul in
+  let x11 = x11 +%^ x15 in
+  let x7 = x7 ^^ x11 in
+  let x7 = x7 <<< 12ul in
+  let x3 = x3 +%^ x7 in
+  let x15 = x15 ^^ x3 in
+  let x15 = x15 <<< 8ul in
+  let x11 = x11 +%^ x15 in
+  let x7 = x7 ^^ x11 in
+  let x7 = x7 <<< 7ul in
+
+  let x0 = x0 +%^ x5 in
+  let x15 = x15 ^^ x0 in
+  let x15 = x15 <<< 16ul in
+  let x10 = x10 +%^ x15 in
+  let x5 = x5 ^^ x10 in
+  let x5 = x5 <<< 12ul in
+  let x0 = x0 +%^ x5 in
+  let x15 = x15 ^^ x0 in
+  let x15 = x15 <<< 8ul in
+  let x10 = x10 +%^ x15 in
+  let x5 = x5 ^^ x10 in
+  let x5 = x5 <<< 7ul in
+
+  let x1 = x1 +%^ x6 in
+  let x12 = x12 ^^ x1 in
+  let x12 = x12 <<< 16ul in
+  let x11 = x11 +%^ x12 in
+  let x6 = x6 ^^ x11 in
+  let x6 = x6 <<< 12ul in
+  let x1 = x1 +%^ x6 in
+  let x12 = x12 ^^ x1 in
+  let x12 = x12 <<< 8ul in
+  let x11 = x11 +%^ x12 in
+  let x6 = x6 ^^ x11 in
+  let x6 = x6 <<< 7ul in
+
+  let x2 = x2 +%^ x7 in
+  let x13 = x13 ^^ x2 in
+  let x13 = x13 <<< 16ul in
+  let x8 = x8 +%^ x13 in
+  let x7 = x7 ^^ x8 in
+  let x7 = x7 <<< 12ul in
+  let x2 = x2 +%^ x7 in
+  let x13 = x13 ^^ x2 in
+  let x13 = x13 <<< 8ul in
+  let x8 = x8 +%^ x13 in
+  let x7 = x7 ^^ x8 in
+  let x7 = x7 <<< 7ul in
+
+  let x3 = x3 +%^ x4 in
+  let x14 = x14 ^^ x3 in
+  let x14 = x14 <<< 16ul in
+  let x9 = x9 +%^ x14 in
+  let x4 = x4 ^^ x9 in
+  let x4 = x4 <<< 12ul in
+  let x3 = x3 +%^ x4 in
+  let x14 = x14 ^^ x3 in
+  let x14 = x14 <<< 8ul in
+  let x9 = x9 +%^ x14 in
+  let x4 = x4 ^^ x9 in
+  let x4 = x4 <<< 7ul in
+
+  (* 4 *)
+
+  let x0 = x0 +%^ x4 in
+  let x12 = x12 ^^ x0 in
+  let x12 = x12 <<< 16ul in
+  let x8 = x8 +%^ x12 in
+  let x4 = x4 ^^ x8 in
+  let x4 = x4 <<< 12ul in
+  let x0 = x0 +%^ x4 in
+  let x12 = x12 ^^ x0 in
+  let x12 = x12 <<< 8ul in
+  let x8 = x8 +%^ x12 in
+  let x4 = x4 ^^ x8 in
+  let x4 = x4 <<< 7ul in
+
+  let x1 = x1 +%^ x5 in
+  let x13 = x13 ^^ x1 in
+  let x13 = x13 <<< 16ul in
+  let x9 = x9 +%^ x13 in
+  let x5 = x5 ^^ x9 in
+  let x5 = x5 <<< 12ul in
+  let x1 = x1 +%^ x5 in
+  let x13 = x13 ^^ x1 in
+  let x13 = x13 <<< 8ul in
+  let x9 = x9 +%^ x13 in
+  let x5 = x5 ^^ x9 in
+  let x5 = x5 <<< 7ul in
+
+  let x2 = x2 +%^ x6 in
+  let x14 = x14 ^^ x2 in
+  let x14 = x14 <<< 16ul in
+  let x10 = x10 +%^ x14 in
+  let x6 = x6 ^^ x10 in
+  let x6 = x6 <<< 12ul in
+  let x2 = x2 +%^ x6 in
+  let x14 = x14 ^^ x2 in
+  let x14 = x14 <<< 8ul in
+  let x10 = x10 +%^ x14 in
+  let x6 = x6 ^^ x10 in
+  let x6 = x6 <<< 7ul in
+
+  let x3 = x3 +%^ x7 in
+  let x15 = x15 ^^ x3 in
+  let x15 = x15 <<< 16ul in
+  let x11 = x11 +%^ x15 in
+  let x7 = x7 ^^ x11 in
+  let x7 = x7 <<< 12ul in
+  let x3 = x3 +%^ x7 in
+  let x15 = x15 ^^ x3 in
+  let x15 = x15 <<< 8ul in
+  let x11 = x11 +%^ x15 in
+  let x7 = x7 ^^ x11 in
+  let x7 = x7 <<< 7ul in
+
+  let x0 = x0 +%^ x5 in
+  let x15 = x15 ^^ x0 in
+  let x15 = x15 <<< 16ul in
+  let x10 = x10 +%^ x15 in
+  let x5 = x5 ^^ x10 in
+  let x5 = x5 <<< 12ul in
+  let x0 = x0 +%^ x5 in
+  let x15 = x15 ^^ x0 in
+  let x15 = x15 <<< 8ul in
+  let x10 = x10 +%^ x15 in
+  let x5 = x5 ^^ x10 in
+  let x5 = x5 <<< 7ul in
+
+  let x1 = x1 +%^ x6 in
+  let x12 = x12 ^^ x1 in
+  let x12 = x12 <<< 16ul in
+  let x11 = x11 +%^ x12 in
+  let x6 = x6 ^^ x11 in
+  let x6 = x6 <<< 12ul in
+  let x1 = x1 +%^ x6 in
+  let x12 = x12 ^^ x1 in
+  let x12 = x12 <<< 8ul in
+  let x11 = x11 +%^ x12 in
+  let x6 = x6 ^^ x11 in
+  let x6 = x6 <<< 7ul in
+
+  let x2 = x2 +%^ x7 in
+  let x13 = x13 ^^ x2 in
+  let x13 = x13 <<< 16ul in
+  let x8 = x8 +%^ x13 in
+  let x7 = x7 ^^ x8 in
+  let x7 = x7 <<< 12ul in
+  let x2 = x2 +%^ x7 in
+  let x13 = x13 ^^ x2 in
+  let x13 = x13 <<< 8ul in
+  let x8 = x8 +%^ x13 in
+  let x7 = x7 ^^ x8 in
+  let x7 = x7 <<< 7ul in
+
+  let x3 = x3 +%^ x4 in
+  let x14 = x14 ^^ x3 in
+  let x14 = x14 <<< 16ul in
+  let x9 = x9 +%^ x14 in
+  let x4 = x4 ^^ x9 in
+  let x4 = x4 <<< 12ul in
+  let x3 = x3 +%^ x4 in
+  let x14 = x14 ^^ x3 in
+  let x14 = x14 <<< 8ul in
+  let x9 = x9 +%^ x14 in
+  let x4 = x4 ^^ x9 in
+  let x4 = x4 <<< 7ul in
+
+  (* 5 *)
+
+  let x0 = x0 +%^ x4 in
+  let x12 = x12 ^^ x0 in
+  let x12 = x12 <<< 16ul in
+  let x8 = x8 +%^ x12 in
+  let x4 = x4 ^^ x8 in
+  let x4 = x4 <<< 12ul in
+  let x0 = x0 +%^ x4 in
+  let x12 = x12 ^^ x0 in
+  let x12 = x12 <<< 8ul in
+  let x8 = x8 +%^ x12 in
+  let x4 = x4 ^^ x8 in
+  let x4 = x4 <<< 7ul in
+
+  let x1 = x1 +%^ x5 in
+  let x13 = x13 ^^ x1 in
+  let x13 = x13 <<< 16ul in
+  let x9 = x9 +%^ x13 in
+  let x5 = x5 ^^ x9 in
+  let x5 = x5 <<< 12ul in
+  let x1 = x1 +%^ x5 in
+  let x13 = x13 ^^ x1 in
+  let x13 = x13 <<< 8ul in
+  let x9 = x9 +%^ x13 in
+  let x5 = x5 ^^ x9 in
+  let x5 = x5 <<< 7ul in
+
+  let x2 = x2 +%^ x6 in
+  let x14 = x14 ^^ x2 in
+  let x14 = x14 <<< 16ul in
+  let x10 = x10 +%^ x14 in
+  let x6 = x6 ^^ x10 in
+  let x6 = x6 <<< 12ul in
+  let x2 = x2 +%^ x6 in
+  let x14 = x14 ^^ x2 in
+  let x14 = x14 <<< 8ul in
+  let x10 = x10 +%^ x14 in
+  let x6 = x6 ^^ x10 in
+  let x6 = x6 <<< 7ul in
+
+  let x3 = x3 +%^ x7 in
+  let x15 = x15 ^^ x3 in
+  let x15 = x15 <<< 16ul in
+  let x11 = x11 +%^ x15 in
+  let x7 = x7 ^^ x11 in
+  let x7 = x7 <<< 12ul in
+  let x3 = x3 +%^ x7 in
+  let x15 = x15 ^^ x3 in
+  let x15 = x15 <<< 8ul in
+  let x11 = x11 +%^ x15 in
+  let x7 = x7 ^^ x11 in
+  let x7 = x7 <<< 7ul in
+
+  let x0 = x0 +%^ x5 in
+  let x15 = x15 ^^ x0 in
+  let x15 = x15 <<< 16ul in
+  let x10 = x10 +%^ x15 in
+  let x5 = x5 ^^ x10 in
+  let x5 = x5 <<< 12ul in
+  let x0 = x0 +%^ x5 in
+  let x15 = x15 ^^ x0 in
+  let x15 = x15 <<< 8ul in
+  let x10 = x10 +%^ x15 in
+  let x5 = x5 ^^ x10 in
+  let x5 = x5 <<< 7ul in
+
+  let x1 = x1 +%^ x6 in
+  let x12 = x12 ^^ x1 in
+  let x12 = x12 <<< 16ul in
+  let x11 = x11 +%^ x12 in
+  let x6 = x6 ^^ x11 in
+  let x6 = x6 <<< 12ul in
+  let x1 = x1 +%^ x6 in
+  let x12 = x12 ^^ x1 in
+  let x12 = x12 <<< 8ul in
+  let x11 = x11 +%^ x12 in
+  let x6 = x6 ^^ x11 in
+  let x6 = x6 <<< 7ul in
+
+  let x2 = x2 +%^ x7 in
+  let x13 = x13 ^^ x2 in
+  let x13 = x13 <<< 16ul in
+  let x8 = x8 +%^ x13 in
+  let x7 = x7 ^^ x8 in
+  let x7 = x7 <<< 12ul in
+  let x2 = x2 +%^ x7 in
+  let x13 = x13 ^^ x2 in
+  let x13 = x13 <<< 8ul in
+  let x8 = x8 +%^ x13 in
+  let x7 = x7 ^^ x8 in
+  let x7 = x7 <<< 7ul in
+
+  let x3 = x3 +%^ x4 in
+  let x14 = x14 ^^ x3 in
+  let x14 = x14 <<< 16ul in
+  let x9 = x9 +%^ x14 in
+  let x4 = x4 ^^ x9 in
+  let x4 = x4 <<< 12ul in
+  let x3 = x3 +%^ x4 in
+  let x14 = x14 ^^ x3 in
+  let x14 = x14 <<< 8ul in
+  let x9 = x9 +%^ x14 in
+  let x4 = x4 ^^ x9 in
+  let x4 = x4 <<< 7ul in
+
+  (* 6 *)
+
+  let x0 = x0 +%^ x4 in
+  let x12 = x12 ^^ x0 in
+  let x12 = x12 <<< 16ul in
+  let x8 = x8 +%^ x12 in
+  let x4 = x4 ^^ x8 in
+  let x4 = x4 <<< 12ul in
+  let x0 = x0 +%^ x4 in
+  let x12 = x12 ^^ x0 in
+  let x12 = x12 <<< 8ul in
+  let x8 = x8 +%^ x12 in
+  let x4 = x4 ^^ x8 in
+  let x4 = x4 <<< 7ul in
+
+  let x1 = x1 +%^ x5 in
+  let x13 = x13 ^^ x1 in
+  let x13 = x13 <<< 16ul in
+  let x9 = x9 +%^ x13 in
+  let x5 = x5 ^^ x9 in
+  let x5 = x5 <<< 12ul in
+  let x1 = x1 +%^ x5 in
+  let x13 = x13 ^^ x1 in
+  let x13 = x13 <<< 8ul in
+  let x9 = x9 +%^ x13 in
+  let x5 = x5 ^^ x9 in
+  let x5 = x5 <<< 7ul in
+
+  let x2 = x2 +%^ x6 in
+  let x14 = x14 ^^ x2 in
+  let x14 = x14 <<< 16ul in
+  let x10 = x10 +%^ x14 in
+  let x6 = x6 ^^ x10 in
+  let x6 = x6 <<< 12ul in
+  let x2 = x2 +%^ x6 in
+  let x14 = x14 ^^ x2 in
+  let x14 = x14 <<< 8ul in
+  let x10 = x10 +%^ x14 in
+  let x6 = x6 ^^ x10 in
+  let x6 = x6 <<< 7ul in
+
+  let x3 = x3 +%^ x7 in
+  let x15 = x15 ^^ x3 in
+  let x15 = x15 <<< 16ul in
+  let x11 = x11 +%^ x15 in
+  let x7 = x7 ^^ x11 in
+  let x7 = x7 <<< 12ul in
+  let x3 = x3 +%^ x7 in
+  let x15 = x15 ^^ x3 in
+  let x15 = x15 <<< 8ul in
+  let x11 = x11 +%^ x15 in
+  let x7 = x7 ^^ x11 in
+  let x7 = x7 <<< 7ul in
+
+  let x0 = x0 +%^ x5 in
+  let x15 = x15 ^^ x0 in
+  let x15 = x15 <<< 16ul in
+  let x10 = x10 +%^ x15 in
+  let x5 = x5 ^^ x10 in
+  let x5 = x5 <<< 12ul in
+  let x0 = x0 +%^ x5 in
+  let x15 = x15 ^^ x0 in
+  let x15 = x15 <<< 8ul in
+  let x10 = x10 +%^ x15 in
+  let x5 = x5 ^^ x10 in
+  let x5 = x5 <<< 7ul in
+
+  let x1 = x1 +%^ x6 in
+  let x12 = x12 ^^ x1 in
+  let x12 = x12 <<< 16ul in
+  let x11 = x11 +%^ x12 in
+  let x6 = x6 ^^ x11 in
+  let x6 = x6 <<< 12ul in
+  let x1 = x1 +%^ x6 in
+  let x12 = x12 ^^ x1 in
+  let x12 = x12 <<< 8ul in
+  let x11 = x11 +%^ x12 in
+  let x6 = x6 ^^ x11 in
+  let x6 = x6 <<< 7ul in
+
+  let x2 = x2 +%^ x7 in
+  let x13 = x13 ^^ x2 in
+  let x13 = x13 <<< 16ul in
+  let x8 = x8 +%^ x13 in
+  let x7 = x7 ^^ x8 in
+  let x7 = x7 <<< 12ul in
+  let x2 = x2 +%^ x7 in
+  let x13 = x13 ^^ x2 in
+  let x13 = x13 <<< 8ul in
+  let x8 = x8 +%^ x13 in
+  let x7 = x7 ^^ x8 in
+  let x7 = x7 <<< 7ul in
+
+  let x3 = x3 +%^ x4 in
+  let x14 = x14 ^^ x3 in
+  let x14 = x14 <<< 16ul in
+  let x9 = x9 +%^ x14 in
+  let x4 = x4 ^^ x9 in
+  let x4 = x4 <<< 12ul in
+  let x3 = x3 +%^ x4 in
+  let x14 = x14 ^^ x3 in
+  let x14 = x14 <<< 8ul in
+  let x9 = x9 +%^ x14 in
+  let x4 = x4 ^^ x9 in
+  let x4 = x4 <<< 7ul in
+
+  (* 7 *)
+
+  let x0 = x0 +%^ x4 in
+  let x12 = x12 ^^ x0 in
+  let x12 = x12 <<< 16ul in
+  let x8 = x8 +%^ x12 in
+  let x4 = x4 ^^ x8 in
+  let x4 = x4 <<< 12ul in
+  let x0 = x0 +%^ x4 in
+  let x12 = x12 ^^ x0 in
+  let x12 = x12 <<< 8ul in
+  let x8 = x8 +%^ x12 in
+  let x4 = x4 ^^ x8 in
+  let x4 = x4 <<< 7ul in
+
+  let x1 = x1 +%^ x5 in
+  let x13 = x13 ^^ x1 in
+  let x13 = x13 <<< 16ul in
+  let x9 = x9 +%^ x13 in
+  let x5 = x5 ^^ x9 in
+  let x5 = x5 <<< 12ul in
+  let x1 = x1 +%^ x5 in
+  let x13 = x13 ^^ x1 in
+  let x13 = x13 <<< 8ul in
+  let x9 = x9 +%^ x13 in
+  let x5 = x5 ^^ x9 in
+  let x5 = x5 <<< 7ul in
+
+  let x2 = x2 +%^ x6 in
+  let x14 = x14 ^^ x2 in
+  let x14 = x14 <<< 16ul in
+  let x10 = x10 +%^ x14 in
+  let x6 = x6 ^^ x10 in
+  let x6 = x6 <<< 12ul in
+  let x2 = x2 +%^ x6 in
+  let x14 = x14 ^^ x2 in
+  let x14 = x14 <<< 8ul in
+  let x10 = x10 +%^ x14 in
+  let x6 = x6 ^^ x10 in
+  let x6 = x6 <<< 7ul in
+
+  let x3 = x3 +%^ x7 in
+  let x15 = x15 ^^ x3 in
+  let x15 = x15 <<< 16ul in
+  let x11 = x11 +%^ x15 in
+  let x7 = x7 ^^ x11 in
+  let x7 = x7 <<< 12ul in
+  let x3 = x3 +%^ x7 in
+  let x15 = x15 ^^ x3 in
+  let x15 = x15 <<< 8ul in
+  let x11 = x11 +%^ x15 in
+  let x7 = x7 ^^ x11 in
+  let x7 = x7 <<< 7ul in
+
+  let x0 = x0 +%^ x5 in
+  let x15 = x15 ^^ x0 in
+  let x15 = x15 <<< 16ul in
+  let x10 = x10 +%^ x15 in
+  let x5 = x5 ^^ x10 in
+  let x5 = x5 <<< 12ul in
+  let x0 = x0 +%^ x5 in
+  let x15 = x15 ^^ x0 in
+  let x15 = x15 <<< 8ul in
+  let x10 = x10 +%^ x15 in
+  let x5 = x5 ^^ x10 in
+  let x5 = x5 <<< 7ul in
+
+  let x1 = x1 +%^ x6 in
+  let x12 = x12 ^^ x1 in
+  let x12 = x12 <<< 16ul in
+  let x11 = x11 +%^ x12 in
+  let x6 = x6 ^^ x11 in
+  let x6 = x6 <<< 12ul in
+  let x1 = x1 +%^ x6 in
+  let x12 = x12 ^^ x1 in
+  let x12 = x12 <<< 8ul in
+  let x11 = x11 +%^ x12 in
+  let x6 = x6 ^^ x11 in
+  let x6 = x6 <<< 7ul in
+
+  let x2 = x2 +%^ x7 in
+  let x13 = x13 ^^ x2 in
+  let x13 = x13 <<< 16ul in
+  let x8 = x8 +%^ x13 in
+  let x7 = x7 ^^ x8 in
+  let x7 = x7 <<< 12ul in
+  let x2 = x2 +%^ x7 in
+  let x13 = x13 ^^ x2 in
+  let x13 = x13 <<< 8ul in
+  let x8 = x8 +%^ x13 in
+  let x7 = x7 ^^ x8 in
+  let x7 = x7 <<< 7ul in
+
+  let x3 = x3 +%^ x4 in
+  let x14 = x14 ^^ x3 in
+  let x14 = x14 <<< 16ul in
+  let x9 = x9 +%^ x14 in
+  let x4 = x4 ^^ x9 in
+  let x4 = x4 <<< 12ul in
+  let x3 = x3 +%^ x4 in
+  let x14 = x14 ^^ x3 in
+  let x14 = x14 <<< 8ul in
+  let x9 = x9 +%^ x14 in
+  let x4 = x4 ^^ x9 in
+  let x4 = x4 <<< 7ul in
+
+  (* 8 *)
+
+  let x0 = x0 +%^ x4 in
+  let x12 = x12 ^^ x0 in
+  let x12 = x12 <<< 16ul in
+  let x8 = x8 +%^ x12 in
+  let x4 = x4 ^^ x8 in
+  let x4 = x4 <<< 12ul in
+  let x0 = x0 +%^ x4 in
+  let x12 = x12 ^^ x0 in
+  let x12 = x12 <<< 8ul in
+  let x8 = x8 +%^ x12 in
+  let x4 = x4 ^^ x8 in
+  let x4 = x4 <<< 7ul in
+
+  let x1 = x1 +%^ x5 in
+  let x13 = x13 ^^ x1 in
+  let x13 = x13 <<< 16ul in
+  let x9 = x9 +%^ x13 in
+  let x5 = x5 ^^ x9 in
+  let x5 = x5 <<< 12ul in
+  let x1 = x1 +%^ x5 in
+  let x13 = x13 ^^ x1 in
+  let x13 = x13 <<< 8ul in
+  let x9 = x9 +%^ x13 in
+  let x5 = x5 ^^ x9 in
+  let x5 = x5 <<< 7ul in
+
+  let x2 = x2 +%^ x6 in
+  let x14 = x14 ^^ x2 in
+  let x14 = x14 <<< 16ul in
+  let x10 = x10 +%^ x14 in
+  let x6 = x6 ^^ x10 in
+  let x6 = x6 <<< 12ul in
+  let x2 = x2 +%^ x6 in
+  let x14 = x14 ^^ x2 in
+  let x14 = x14 <<< 8ul in
+  let x10 = x10 +%^ x14 in
+  let x6 = x6 ^^ x10 in
+  let x6 = x6 <<< 7ul in
+
+  let x3 = x3 +%^ x7 in
+  let x15 = x15 ^^ x3 in
+  let x15 = x15 <<< 16ul in
+  let x11 = x11 +%^ x15 in
+  let x7 = x7 ^^ x11 in
+  let x7 = x7 <<< 12ul in
+  let x3 = x3 +%^ x7 in
+  let x15 = x15 ^^ x3 in
+  let x15 = x15 <<< 8ul in
+  let x11 = x11 +%^ x15 in
+  let x7 = x7 ^^ x11 in
+  let x7 = x7 <<< 7ul in
+
+  let x0 = x0 +%^ x5 in
+  let x15 = x15 ^^ x0 in
+  let x15 = x15 <<< 16ul in
+  let x10 = x10 +%^ x15 in
+  let x5 = x5 ^^ x10 in
+  let x5 = x5 <<< 12ul in
+  let x0 = x0 +%^ x5 in
+  let x15 = x15 ^^ x0 in
+  let x15 = x15 <<< 8ul in
+  let x10 = x10 +%^ x15 in
+  let x5 = x5 ^^ x10 in
+  let x5 = x5 <<< 7ul in
+
+  let x1 = x1 +%^ x6 in
+  let x12 = x12 ^^ x1 in
+  let x12 = x12 <<< 16ul in
+  let x11 = x11 +%^ x12 in
+  let x6 = x6 ^^ x11 in
+  let x6 = x6 <<< 12ul in
+  let x1 = x1 +%^ x6 in
+  let x12 = x12 ^^ x1 in
+  let x12 = x12 <<< 8ul in
+  let x11 = x11 +%^ x12 in
+  let x6 = x6 ^^ x11 in
+  let x6 = x6 <<< 7ul in
+
+  let x2 = x2 +%^ x7 in
+  let x13 = x13 ^^ x2 in
+  let x13 = x13 <<< 16ul in
+  let x8 = x8 +%^ x13 in
+  let x7 = x7 ^^ x8 in
+  let x7 = x7 <<< 12ul in
+  let x2 = x2 +%^ x7 in
+  let x13 = x13 ^^ x2 in
+  let x13 = x13 <<< 8ul in
+  let x8 = x8 +%^ x13 in
+  let x7 = x7 ^^ x8 in
+  let x7 = x7 <<< 7ul in
+
+  let x3 = x3 +%^ x4 in
+  let x14 = x14 ^^ x3 in
+  let x14 = x14 <<< 16ul in
+  let x9 = x9 +%^ x14 in
+  let x4 = x4 ^^ x9 in
+  let x4 = x4 <<< 12ul in
+  let x3 = x3 +%^ x4 in
+  let x14 = x14 ^^ x3 in
+  let x14 = x14 <<< 8ul in
+  let x9 = x9 +%^ x14 in
+  let x4 = x4 ^^ x9 in
+  let x4 = x4 <<< 7ul in
+
+  (* 9 *)
+
+  let x0 = x0 +%^ x4 in
+  let x12 = x12 ^^ x0 in
+  let x12 = x12 <<< 16ul in
+  let x8 = x8 +%^ x12 in
+  let x4 = x4 ^^ x8 in
+  let x4 = x4 <<< 12ul in
+  let x0 = x0 +%^ x4 in
+  let x12 = x12 ^^ x0 in
+  let x12 = x12 <<< 8ul in
+  let x8 = x8 +%^ x12 in
+  let x4 = x4 ^^ x8 in
+  let x4 = x4 <<< 7ul in
+
+  let x1 = x1 +%^ x5 in
+  let x13 = x13 ^^ x1 in
+  let x13 = x13 <<< 16ul in
+  let x9 = x9 +%^ x13 in
+  let x5 = x5 ^^ x9 in
+  let x5 = x5 <<< 12ul in
+  let x1 = x1 +%^ x5 in
+  let x13 = x13 ^^ x1 in
+  let x13 = x13 <<< 8ul in
+  let x9 = x9 +%^ x13 in
+  let x5 = x5 ^^ x9 in
+  let x5 = x5 <<< 7ul in
+
+  let x2 = x2 +%^ x6 in
+  let x14 = x14 ^^ x2 in
+  let x14 = x14 <<< 16ul in
+  let x10 = x10 +%^ x14 in
+  let x6 = x6 ^^ x10 in
+  let x6 = x6 <<< 12ul in
+  let x2 = x2 +%^ x6 in
+  let x14 = x14 ^^ x2 in
+  let x14 = x14 <<< 8ul in
+  let x10 = x10 +%^ x14 in
+  let x6 = x6 ^^ x10 in
+  let x6 = x6 <<< 7ul in
+
+  let x3 = x3 +%^ x7 in
+  let x15 = x15 ^^ x3 in
+  let x15 = x15 <<< 16ul in
+  let x11 = x11 +%^ x15 in
+  let x7 = x7 ^^ x11 in
+  let x7 = x7 <<< 12ul in
+  let x3 = x3 +%^ x7 in
+  let x15 = x15 ^^ x3 in
+  let x15 = x15 <<< 8ul in
+  let x11 = x11 +%^ x15 in
+  let x7 = x7 ^^ x11 in
+  let x7 = x7 <<< 7ul in
+
+  let x0 = x0 +%^ x5 in
+  let x15 = x15 ^^ x0 in
+  let x15 = x15 <<< 16ul in
+  let x10 = x10 +%^ x15 in
+  let x5 = x5 ^^ x10 in
+  let x5 = x5 <<< 12ul in
+  let x0 = x0 +%^ x5 in
+  let x15 = x15 ^^ x0 in
+  let x15 = x15 <<< 8ul in
+  let x10 = x10 +%^ x15 in
+  let x5 = x5 ^^ x10 in
+  let x5 = x5 <<< 7ul in
+
+  let x1 = x1 +%^ x6 in
+  let x12 = x12 ^^ x1 in
+  let x12 = x12 <<< 16ul in
+  let x11 = x11 +%^ x12 in
+  let x6 = x6 ^^ x11 in
+  let x6 = x6 <<< 12ul in
+  let x1 = x1 +%^ x6 in
+  let x12 = x12 ^^ x1 in
+  let x12 = x12 <<< 8ul in
+  let x11 = x11 +%^ x12 in
+  let x6 = x6 ^^ x11 in
+  let x6 = x6 <<< 7ul in
+
+  let x2 = x2 +%^ x7 in
+  let x13 = x13 ^^ x2 in
+  let x13 = x13 <<< 16ul in
+  let x8 = x8 +%^ x13 in
+  let x7 = x7 ^^ x8 in
+  let x7 = x7 <<< 12ul in
+  let x2 = x2 +%^ x7 in
+  let x13 = x13 ^^ x2 in
+  let x13 = x13 <<< 8ul in
+  let x8 = x8 +%^ x13 in
+  let x7 = x7 ^^ x8 in
+  let x7 = x7 <<< 7ul in
+
+  let x3 = x3 +%^ x4 in
+  let x14 = x14 ^^ x3 in
+  let x14 = x14 <<< 16ul in
+  let x9 = x9 +%^ x14 in
+  let x4 = x4 ^^ x9 in
+  let x4 = x4 <<< 12ul in
+  let x3 = x3 +%^ x4 in
+  let x14 = x14 ^^ x3 in
+  let x14 = x14 <<< 8ul in
+  let x9 = x9 +%^ x14 in
+  let x4 = x4 ^^ x9 in
+  let x4 = x4 <<< 7ul in
+ 
+  (* (\* 10 *\) *)
+  (* let x0 = x.(0ul) in *)
+  (* let x1 = x.(1ul) in *)
+  (* let x2 = x.(2ul) in *)
+  (* let x3 = x.(3ul) in *)
+  (* let x4 = x.(4ul) in *)
+  (* let x5 = x.(5ul) in *)
+  (* let x6 = x.(6ul) in *)
+  (* let x7 = x.(7ul) in *)
+  (* let x8 = x.(8ul) in *)
+  (* let x9 = x.(9ul) in *)
+  (* let x10 = x.(10ul) in *)
+  (* let x11 = x.(11ul) in *)
+  (* let x12 = x.(12ul) in *)
+  (* let x13 = x.(13ul) in *)
+  (* let x14 = x.(14ul) in *)
+  (* let x15 = x.(15ul) in *)
+
+  let x0 = x0 +^ j0 in
+  let x1 = x1 +^ j1 in
+  let x2 = x2 +^ j2 in
+  let x3 = x3 +^ j3 in
+  let x4 = x4 +^ j4 in
+  let x5 = x5 +^ j5 in
+  let x6 = x6 +^ j6 in
+  let x7 = x7 +^ j7 in
+  let x8 = x8 +^ j8 in
+  let x9 = x9 +^ j9 in
+  let x10 = x10 +^ j10 in
+  let x11 = x11 +^ j11 in
+  let x12 = x12 +^ j12 in
+  let x13 = x13 +^ j13 in
+  let x14 = x14 +^ j14 in
+  let x15 = x15 +^ j15 in
+
+  let open FStar.Buffer in
+  let m0 = load32_le (sub m 0ul 4ul) in
+  let m1 = load32_le (sub m 4ul 4ul) in
+  let m2 = load32_le (sub m 8ul 4ul) in
+  let m3 = load32_le (sub m 12ul 4ul) in
+  let m4 = load32_le (sub m 16ul 4ul) in
+  let m5 = load32_le (sub m 20ul 4ul) in
+  let m6 = load32_le (sub m 24ul 4ul) in
+  let m7 = load32_le (sub m 28ul 4ul) in
+  let m8 = load32_le (sub m 32ul 4ul) in
+  let m9 = load32_le (sub m 36ul 4ul) in
+  let m10 = load32_le (sub m 40ul 4ul) in
+  let m11 = load32_le (sub m 44ul 4ul) in
+  let m12 = load32_le (sub m 48ul 4ul) in
+  let m13 = load32_le (sub m 52ul 4ul) in
+  let m14 = load32_le (sub m 56ul 4ul) in
+  let m15 = load32_le (sub m 60ul 4ul) in
+
+  let x0 = x0 ^^ m0 in
+  let x1 = x1 ^^ m1 in
+  let x2 = x2 ^^ m2 in
+  let x3 = x3 ^^ m3 in
+  let x4 = x4 ^^ m4 in
+  let x5 = x5 ^^ m5 in
+  let x6 = x6 ^^ m6 in
+  let x7 = x7 ^^ m7 in
+  let x8 = x8 ^^ m8 in
+  let x9 = x9 ^^ m9 in
+  let x10 = x10 ^^ m10 in
+  let x11 = x11 ^^ m11 in
+  let x12 = x12 ^^ m12 in
+  let x13 = x13 ^^ m13 in
+  let x14 = x14 ^^ m14 in
+  let x15 = x15 ^^ m15 in
+
+  store32_le (sub c 0ul 4ul) x0;
+  store32_le (sub c 4ul 4ul) x1;
+  store32_le (sub c 8ul 4ul) x2;
+  store32_le (sub c 12ul 4ul) x3;
+  store32_le (sub c 16ul 4ul) x4;
+  store32_le (sub c 20ul 4ul) x5;
+  store32_le (sub c 24ul 4ul) x6;
+  store32_le (sub c 28ul 4ul) x7;
+  store32_le (sub c 32ul 4ul) x8;
+  store32_le (sub c 36ul 4ul) x9;
+  store32_le (sub c 40ul 4ul) x10;
+  store32_le (sub c 44ul 4ul) x11;
+  store32_le (sub c 48ul 4ul) x12;
+  store32_le (sub c 52ul 4ul) x13;
+  store32_le (sub c 56ul 4ul) x14;
+  store32_le (sub c 60ul 4ul) x15
+
+
+val chacha_encrypt_bytes_loop:
+  ctx:chacha_ctx ->
+  m:uint8_p ->
+  c:uint8_p ->
+  len:UInt32.t ->
+  Stack unit
+    (requires (fun _ -> True))
+    (ensures  (fun _ _ _ -> True))
+let rec chacha_encrypt_bytes_loop ctx m c len =
+  if FStar.UInt32 (len <^ 64ul) then ()
+  else (
+    chacha_encrypt_bytes_core ctx m c;
+    let ctr = ctx.(12ul) in
+    ctx.(12ul) <- FStar.UInt32 (ctr +^ 1ul);
+    chacha_encrypt_bytes_loop ctx (offset m 64ul) (offset c 64ul) (FStar.UInt32 (len -^ 64ul))
+  )
+
+
+module U32 = FStar.UInt32
+
+val chacha_encrypt_bytes:
+  ctx:chacha_ctx ->
+  m:uint8_p ->
+  c:uint8_p ->
+  len:UInt32.t ->
+  Stack unit
+    (requires (fun _ -> True))
+    (ensures  (fun _ _ _ -> True))
+let rec chacha_encrypt_bytes ctx m c len =
+  push_frame();
+  chacha_encrypt_bytes_loop ctx m c len;
+  let rem = U32 (len &^ 63ul) in // % 64
+  let q   = U32 (len >>^ 6ul) in // / 64
+  if FStar.UInt32 (rem >=^ 0ul) then (
+    let tmp = create (0uy) 64ul in
+    let m = offset m (U32 (len -^ rem)) in
+    let c = offset c (U32 (len -^ rem)) in
+    blit m 0ul tmp 0ul rem;
+    chacha_encrypt_bytes_core ctx tmp tmp;
+    blit tmp 0ul c 0ul rem );
+  pop_frame()
+
+
+
+(* // Concrete implementation of CHACHA20 and countermode encryption *)
+(* // Not much point verifying its against a more complex pure specification. *)
+
+(* open FStar.Mul *)
+(* open FStar.Ghost *)
+(* (\*  Machine integers *\) *)
+(* open FStar.UInt8 *)
+(* open FStar.UInt32 *)
+(* open FStar.Int.Cast *)
+(* (\*  Effects and memory layout *\) *)
+(* open FStar.HyperStack *)
+(* (\*  Buffers *\) *)
+(* open FStar.Buffer *)
+(* open Buffer.Utils *)
+
+(* module HH = FStar.HyperHeap *)
+(* module HS = FStar.HyperStack *)
+
+(* type u64 = FStar.UInt64.t *)
+
+
+(* (\*** Chacha 20 ***\) *)
+
+(* inline_for_extraction let keylen   = 32ul *)
+(* inline_for_extraction let blocklen = 64ul  *)
+(* inline_for_extraction let ivlen    = 12ul *)
+
+(* type lbytes l = b:bytes {length b = l} *)
+(* type key   = lbytes (v keylen) *)
+(* type block = lbytes (v blocklen) *)
+(* type iv    = lbytes (v ivlen) *)
+
+(* // internally, blocks are represented as 16 x 4-byte integers *)
+(* private type matrix = m:uint32s{length m = v blocklen / 4} *)
+
+(* private type shuffle =  *)
+(*   m:matrix -> STL unit *)
+(*   (requires (fun h -> live h m)) *)
+(*   (ensures (fun h0 _ h1 -> live h1 m /\ modifies_1 m h0 h1 )) *)
+
+(* (\* lifted by hand for now: *\) *)
+(* private val line: *)
+(*   m:matrix ->  *)
+(*   a:u32{v a < 16} ->  *)
+(*   b:u32{v b < 16} ->  *)
+(*   d:u32{v d < 16} ->  *)
+(*   s:u32{v s <= 32}-> STL unit *)
+(*   (requires (fun h -> live h m)) *)
+(*   (ensures (fun h0 _ h1 -> live h1 m /\ modifies_1 m h0 h1 )) *)
+(* let line m a b d s =  *)
+(*   m.(a) <- m.(a) +%^ m.(b); *)
+(*   m.(d) <-(m.(d) ^^  m.(a)) <<< s *)
+
+(* private val quarter_round: *)
+(*   m:matrix ->  *)
+(*   a:u32{v a < 16} ->  *)
+(*   b:u32{v b < 16} ->  *)
+(*   c:u32{v c < 16} ->  *)
+(*   d:u32{v d < 16} -> STL unit *)
+(*   (requires (fun h -> live h m)) *)
+(*   (ensures (fun h0 _ h1 -> live h1 m /\ modifies_1 m h0 h1 )) *)
+(* let quarter_round m a b c d =  *)
+(* (\* *)
+(*   let line a b d s =  *)
+(*     upd m a (m.(a) +%^ m.(b)); *)
+(*     upd m d((m.(d) ^^  m.(a)) <<< s) in *)
+(* *\)     *)
+(*   line m a b d 16ul; *)
+(*   line m c d b 12ul; *)
+(*   line m a b d  8ul;  *)
+(*   line m c d b  7ul *)
+
+(* private val column_round: shuffle  *)
+(* let column_round m = *)
+(*   quarter_round m 0ul 4ul  8ul 12ul; *)
+(*   quarter_round m 1ul 5ul  9ul 13ul; *)
+(*   quarter_round m 2ul 6ul 10ul 14ul; *)
+(*   quarter_round m 3ul 7ul 11ul 15ul *)
+
+(* private val diagonal_round: shuffle *)
+(* let diagonal_round m = *)
+(*   quarter_round m 0ul 5ul 10ul 15ul; *)
+(*   quarter_round m 1ul 6ul 11ul 12ul; *)
+(*   quarter_round m 2ul 7ul  8ul 13ul; *)
+(*   quarter_round m 3ul 4ul  9ul 14ul *)
+
+(* private val rounds: shuffle  *)
+(* let rounds m = (\* 20 rounds *\) *)
+(*   column_round m; diagonal_round m;  *)
+(*   column_round m; diagonal_round m; *)
+(*   column_round m; diagonal_round m; *)
+(*   column_round m; diagonal_round m; *)
+(*   column_round m; diagonal_round m; *)
+(*   column_round m; diagonal_round m; *)
+(*   column_round m; diagonal_round m; *)
+(*   column_round m; diagonal_round m; *)
+(*   column_round m; diagonal_round m; *)
+(*   column_round m; diagonal_round m *)
+
+(* private val chacha20_init:  *)
+(*   m:matrix -> k:key{disjoint m k} -> n:iv{disjoint m n} -> counter:u32 ->  *)
+(*   STL unit *)
+(*   (requires (fun h -> live h m /\ live h k /\ live h n )) *)
+(*   (ensures (fun h0 _ h1 -> live h1 m /\ modifies_1 m h0 h1)) *)
+
+(* private val fill: m:matrix -> i:u32 -> len:u32 {v i + v len <= 16}-> src:bytes {length src = 4 * v len} ->  *)
+(*   STL unit *)
+(*   (requires (fun h -> live h m /\ live h src /\ disjoint m src)) *)
+(*   (ensures (fun h0 _ h1 -> live h1 m /\ modifies_1 m h0 h1)) *)
+(* let rec fill m i len src = *)
+(*   if len <> 0ul then ( *)
+(*     m.(i) <- uint32_of_bytes (sub src 0ul 4ul);  *)
+(*     let len = len -^ 1ul in  *)
+(*     fill m (i +^ 1ul) len (sub src 4ul (4ul *^ len))) *)
+
+(* //review handling of endianness *)
+
+(* // RFC 7539 2.3 *)
+(* let chacha20_init m key iv counter = *)
+(*   m.(0ul) <- 0x61707865ul; *)
+(*   m.(1ul) <- 0x3320646eul; *)
+(*   m.(2ul) <- 0x79622d32ul; *)
+(*   m.(3ul) <- 0x6b206574ul; *)
+(*   fill m 4ul 8ul key; *)
+(*   m.(12ul) <- counter;  *)
+(*   fill m 13ul 3ul iv *)
+
+(* (\* lifted by hand for now: *\) *)
+(* private val add:  *)
+(*   m: matrix -> m0: matrix{disjoint m m0} ->  *)
+(*   i:u32 { i <^ 16ul } -> *)
+(*   STL unit *)
+(*   (requires (fun h -> live h m /\ live h m0)) *)
+(*   (ensures (fun h0 _ h1 -> live h1 m /\ modifies_1 m h0 h1)) *)
+(* let add m m0 i =  *)
+(*   m.(i) <- m.(i) +%^ m0.(i) *)
+
+(* private val sum_matrixes:  *)
+(*   m: matrix -> m0:matrix{disjoint m m0} ->  *)
+(*   STL unit *)
+(*   (requires (fun h -> live h m /\ live h m0)) *)
+(*   (ensures (fun h0 _ h1 -> live h1 m /\ modifies_1 m h0 h1)) *)
+(* let sum_matrixes m m0 = *)
+(* //let add i = upd m i (m.(i) +%^ m0.(i)) in // inlined?  *)
+(* // forUint32 0ul 15ul (fun i -> add m m0 i) *)
+(*   add m m0  0ul; *)
+(*   add m m0  1ul; *)
+(*   add m m0  2ul; *)
+(*   add m m0  3ul; *)
+(*   add m m0  4ul; *)
+(*   add m m0  5ul; *)
+(*   add m m0  6ul; *)
+(*   add m m0  7ul; *)
+(*   add m m0  8ul; *)
+(*   add m m0  9ul; *)
+(*   add m m0 10ul; *)
+(*   add m m0 11ul; *)
+(*   add m m0 12ul; *)
+(*   add m m0 13ul; *)
+(*   add m m0 14ul; *)
+(*   add m m0 15ul *)
+
+(* private val chacha20_update:  *)
+(*   output:bytes ->  *)
+(*   state:uint32s{length state = 32 /\ disjoint state output} -> *)
+(*   len:u32{v len <= 64 /\ length output >= v len} -> STL unit *)
+(*     (requires (fun h -> live h state /\ live h output)) *)
+(*     (ensures (fun h0 _ h1 -> live h1 output /\ live h1 state /\ modifies_2 output state h0 h1 )) *)
+(* let chacha20_update output state len = *)
+(*   (\* Initial state *\)  *)
+(*   let m  = sub state  0ul 16ul in *)
+(*   let m0 = sub state 16ul 16ul in // do we ever rely on m and m0 being contiguous? *)
+(*   blit m 0ul m0 0ul 16ul; *)
+(*   rounds m; *)
+(*   (\* Sum the matrixes *\) *)
+(*   sum_matrixes m m0; *)
+(*   (\* Serialize the state into byte stream *\) *)
+(*   bytes_of_uint32s output m len *)
+(* // avoid this copy when XORing? merge the sum_matrix and output loops? we don't use m0 afterward.  *)
+
+(* // computes one pseudo-random 64-byte block  *)
+(* // (consider fixing len to 64ul) *)
+
+(* val chacha20:  *)
+(*   output:bytes ->  *)
+(*   k:key -> *)
+(*   n:iv -> *)
+(*   counter: u32 -> *)
+(*   len:u32{v len <= v blocklen /\ v len <= length output} -> STL unit *)
+(*     (requires (fun h -> live h k /\ live h n /\ live h output)) *)
+(*     (ensures (fun h0 _ h1 -> live h1 output /\ modifies_1 output h0 h1 )) *)
+(* let chacha20 output key n counter len =  *)
+(*   push_frame (); *)
+(*   let state = create 0ul 32ul in *)
+(*   let m = sub state 0ul 16ul in *)
+(*   chacha20_init m key n counter; *)
+(*   chacha20_update output state len; *)
+(*   pop_frame () *)
+
+(* // Performance: it may be easier to precompute and re-use an expanded key (m0),  *)
+(* // to avoid passing around (key, counter, iv, constant), and only have m on the stack. *)
+(* // We may also merge the 3 final loops: sum_matrixes, bytes_of_uint32s, and outer XOR/ADD.  *)
+
+
+(* (\*** Counter-mode Encryption ***\) *)
+
+(* // The rest of this code is not specific to chacha20. *)
+(* // It is parameterized by the initial counter (0, or 1 for some AEAD) *)
+(* // and the block length (here 64 bytes). *)
+(* // It should appear after PRF idealization. *)
+
+(* private let prf = chacha20 *)
+
+(* // XOR-based encryption and decryption (just swap ciphertext and plaintext) *)
+(* val counter_mode:  *)
+(*   k:key -> n:iv -> counter:u32 ->  *)
+(*   len:u32{v counter + v len / v blocklen < pow2 32} -> *)
+(*   plaintext:bytes {length plaintext = v len /\ disjoint k plaintext} ->  *)
+(*   ciphertext:bytes {length ciphertext = v len /\ disjoint n ciphertext /\ disjoint k ciphertext /\ disjoint plaintext ciphertext} ->  *)
+(*   STL unit *)
+(*     (requires (fun h -> live h ciphertext /\ live h k /\ live h n /\ live h plaintext)) *)
+(*     (ensures (fun h0 _ h1 -> live h1 ciphertext /\ modifies_1 ciphertext h0 h1)) *)
+
+(* #reset-options "--z3timeout 100" *)
+(* // a bit slow, e.g. on the len precondition *)
+
+(* let rec counter_mode key iv counter len plaintext ciphertext = *)
+(*   if len =^ 0ul then ()  *)
+(*   else if len <^ blocklen  *)
+(*   then (\* encrypt final partial block *\) *)
+(*     begin *)
+(*       let cipher = sub ciphertext  0ul len in  *)
+(*       let plain  = sub plaintext   0ul len in  *)
+(*       prf cipher key iv counter len; *)
+(*       xor_bytes_inplace cipher plain len *)
+(*     end *)
+(*   else (\* encrypt full block *\) *)
+(*     begin *)
+(*       let cipher = sub ciphertext  0ul blocklen in *)
+(*       let plain  = sub plaintext   0ul blocklen in *)
+(*       prf cipher key iv counter blocklen; *)
+(*       xor_bytes_inplace cipher plain blocklen; *)
+(*       let len = len -^ blocklen in *)
+(*       let ciphertext = sub ciphertext blocklen len in *)
+(*       let plaintext  = sub plaintext  blocklen len in *)
+(*       counter_mode key iv (counter +^ 1ul) len plaintext ciphertext *)
+(*     end *)
 
